WIP
WIP

WIP

WIP

WIP

WIP

WIP

Debugging

WIP

WIP

WIP

WIP

WIP

WIP

WIP

WIP

WIP

WIP

WIP

WIP

WIP

WIP

WIP

WIP

WIP

WIP

WIP

WIP

WIP

WIP

WIP

WIP

Add bound_op

WIP

WIP

WIP

copy_bounds, fill_template

WIP

WIP

WIP

Fix bugs in shr

WIP

WIP

copy_bounds, fill_templates

Add LadderStepDisplay

copy_bounds

Add more notations

Copy bounds

Fix bounds

More notations

C code

More notations for fewer casts

Update log, fix shr

Don't insert identity casts

Update log with elimination of identity casts

Remove useless + casts

Remove useless & casts

Update 32-bit ladder step

Various small notation fixes

Add print of 32-bit ladder

Fix binary notation in 32-bit

Update notations

Update MulDisplay

Add display target

Update notations import

Update notations import

Update display target

Add a bunch of C display files

Remove lowercase files

Add MapBounds

Add 41417 MulDisplay

WIP

Add ComputeBounds

WIP

More/better C notations

Some binary things, remove extra notation

Add Java notations

Remove Java

Hopefully better java display targets

Add Java display things

Add more java display

Add src/SpecificGen/GF25519_64Reflective/Reified/LadderStepJavaDisplay.log

Add more java logs

Constant notation fixes

Add comment about Java casts

davidben tells me unsigned short is bigger than uint8_t

More notations fixes

Fix constants in display

Add more java display

Update display

WIP

WIP

Add TODO

Update TODO

Add to TODO

WIP on good bounds

WIP on good bounds

WIP on good bounds

WIP

WIP

WIP

WIP

Add Z.log2_up_nonneg to zarith

Add valid_update lemmas about FixedWordSizes

src/Reflection/Equality.v
@@ -33,7 +33,6 @@ Section language.
            | [ |- Prod _ _ = Prod _ _ ] => apply f_equal2
            | [ |- Arrow _ _ = Arrow _ _ ] => apply f_equal2
            | [ |- Tbase _ = Tbase _ ] => apply f_equal
-           | [ |- Tflat _ = Tflat _ ] => apply f_equal
            | [ H : forall Y, _ = true -> _ = Y |- _ = ?Y' ]
              => is_var Y'; apply H; solve [ t ]
            | [ H : forall X Y, X = Y -> _ = true |- _ = true ]
@@ -59,13 +58,9 @@ Section language.
        | right pf => right (fun pf' => let pf'' := eq_sym (flat_type_dec_lb _ _ pf') in
                                        Bool.diff_true_false (eq_trans pf'' pf))
        end.
-  Fixpoint type_beq (X Y : type) {struct X} : bool
+  Definition type_beq (X Y : type) : bool
     := match X, Y with
-       | Tflat T, Tflat T0 => flat_type_beq T T0
-       | Arrow A B, Arrow A0 B0 => (eq_base_type_code A A0 && type_beq B B0)%bool
-       | Tflat _, _
-       | Arrow _ _, _
-         => false
+       | Arrow A B, Arrow A0 B0 => (flat_type_beq A A0 && flat_type_beq B B0)%bool
        end.
   Lemma type_dec_bl X : forall Y, type_beq X Y = true -> X = Y.
   Proof. clear base_type_code_lb; pose proof flat_type_dec_bl; induction X, Y; t. Defined.
@@ -143,36 +138,18 @@ Section encode_decode.
   Proof. intro p; specialize (f (flat_type_encode p)); destruct t1, p; exact f. Defined.
 
   Definition type_code (t1 t2 : type)
-    := match t1, t2 with
-       | Tflat T1, Tflat T2 => T1 = T2
-       | Arrow A1 B1, Arrow A2 B2 => A1 = A2 /\ B1 = B2
-       | Tflat _, _
-       | Arrow _ _, _
-         => False
-       end.
+    := domain t1 = domain t2 /\ codomain t1 = codomain t2.
   Definition type_encode {t1 t2} : t1 = t2 -> type_code t1 t2
-    := match t1, t2 return t1 = t2 -> type_code t1 t2 with
-       | Tflat T1, Tflat T2 => fun H => match H with eq_refl => eq_refl end
-       | Arrow A1 B1, Arrow A2 B2
-         => fun H => conj (match H with eq_refl => eq_refl end)
-                          (match H with eq_refl => eq_refl end)
-       | Tflat _, _
-       | Arrow _ _, _
-         => fun H => match H with eq_refl => I end
-       end.
+    := fun H => conj (f_equal _ H) (f_equal _ H).
   Definition type_decode {t1 t2} : type_code t1 t2 -> t1 = t2
     := match t1, t2 return type_code t1 t2 -> t1 = t2 with
-       | Tflat T1, Tflat T2 => fun H => f_equal Tflat H
        | Arrow A1 B1, Arrow A2 B2
          => fun H => f_equal2 Arrow (let (a, b) := H in a) (let (a, b) := H in b)
-       | Tflat _, _
-       | Arrow _ _, _
-         => fun H : False => match H with end
        end.
   Lemma type_endecode {t1 t2} H : type_decode (@type_encode t1 t2 H) = H.
   Proof. subst t2; destruct t1; reflexivity. Defined.
   Lemma type_deencode {t1 t2} H : type_encode (@type_decode t1 t2 H) = H.
-  Proof. destruct t1, t2; destruct H; subst; reflexivity. Defined.
+  Proof. destruct t1, t2; destruct H; simpl in *; subst; reflexivity. Defined.
 
   Definition path_type_rect {t1 t2 : type} (P : t1 = t2 -> Type)
              (f : forall p, P (type_decode p))
@@ -209,10 +186,6 @@ Ltac inversion_flat_type := repeat inversion_flat_type_step.
 
 Ltac inversion_type_step :=
   lazymatch goal with
-  | [ H : _ = Tflat _ |- _ ]
-    => induction_type_in_using H @path_type_rect
-  | [ H : Tflat _ = _ |- _ ]
-    => induction_type_in_using H @path_type_rect
   | [ H : _ = Arrow _ _ |- _ ]
     => induction_type_in_using H @path_type_rect
   | [ H : Arrow _ _ = _ |- _ ]
