src/Specific/GF25519Reflective/Reified/Pack.v
@@ -1,17 +1,17 @@
-Require Import Crypto.Specific.GF25519Reflective.CommonUnOpFEToWire.
+Require Import Crypto.Specific.GF25519Reflective.Common.
 
 Definition rpackZ_sig : rexpr_unop_FEToWire_sig pack. Proof. reify_sig. Defined.
-Definition rpackW := Eval vm_compute in rword_of_Z rpackZ_sig.
-Lemma rpackW_correct_and_bounded_gen : correct_and_bounded_genT rpackW rpackZ_sig.
+Definition rpackZ := Eval vm_compute in proj1_sig rpackZ_sig.
+Lemma rpackZ_correct_and_bounded_gen : correct_and_bounded_genT rpackZ rpackZ_sig.
 Proof. rexpr_correct. Qed.
-Definition rpack_output_bounds := Eval vm_compute in compute_bounds rpackW ExprUnOpFEToWire_bounds.
+Definition rpack_output_bounds := Eval vm_compute in compute_bounds rpackZ ExprUnOpFEToWire_bounds.
 Local Obligation Tactic := intros; vm_compute; constructor.
-Program Definition rpackW_correct_and_bounded
+Program Definition rpackZ_correct_and_bounded
   := ExprUnOpFEToWire_correct_and_bounded
-       rpackW pack rpackZ_sig rpackW_correct_and_bounded_gen
+       rpackZ pack rpackZ_sig rpackZ_correct_and_bounded_gen
        _ _.
 
 Local Open Scope string_scope.
-Compute ("Pack", compute_bounds_for_display rpackW ExprUnOpFEToWire_bounds).
-Compute ("Pack overflows? ", sanity_compute rpackW ExprUnOpFEToWire_bounds).
-Compute ("Pack overflows (error if it does)? ", sanity_check rpackW ExprUnOpFEToWire_bounds).
+Compute ("Pack", compute_bounds_for_display rpackZ ExprUnOpFEToWire_bounds).
+Compute ("Pack overflows? ", sanity_compute rpackZ ExprUnOpFEToWire_bounds).
+Compute ("Pack overflows (error if it does)? ", sanity_check rpackZ ExprUnOpFEToWire_bounds).
