src/Reflection/Eta.v
@@ -1,0 +1,39 @@
+Require Import Crypto.Reflection.Syntax.
+Require Import Crypto.Reflection.ExprInversion.
+
+Section language.
+  Context {base_type_code : Type}
+          {op : flat_type base_type_code -> flat_type base_type_code -> Type}.
+  Local Notation Expr := (@Expr base_type_code op).
+  Section with_var.
+    Context {var : base_type_code -> Type}.
+    Local Notation exprf := (@exprf base_type_code op var).
+    Local Notation expr := (@expr base_type_code op var).
+    Fixpoint interp_flat_type_eta {t T} : (interp_flat_type var t -> T) -> interp_flat_type var t -> T
+      := match t return (interp_flat_type var t -> T) -> interp_flat_type var t -> T with
+         | Tbase T => fun f => f
+         | Unit => fun f => f
+         | Prod A B
+           => fun f x
+              => let '(a, b) := x in
+                 @interp_flat_type_eta
+                   A _
+                   (fun a' => @interp_flat_type_eta B _ (fun b' => f (a', b')) b)
+                   a
+         end.
+    Fixpoint exprf_eta {t} (e : exprf t) : exprf t
+      := match e in Syntax.exprf _ _ t return exprf t with
+         | TT => TT
+         | Var t v => Var v
+         | Op t1 tR opc args => Op opc (@exprf_eta _ args)
+         | LetIn tx ex tC eC
+           => LetIn (@exprf_eta _ ex)
+                    (interp_flat_type_eta eC)
+         | Pair tx ex ty ey => Pair (@exprf_eta _ ex) (@exprf_eta _ ey)
+         end.
+    Definition expr_eta {t} (e : expr t) : expr (Arrow (domain t) (codomain t))
+      := Abs (interp_flat_type_eta (fun x => exprf_eta (invert_Abs e x))).
+  End with_var.
+  Definition ExprEta {t} (e : Expr t) : Expr (Arrow (domain t) (codomain t))
+    := fun var => expr_eta (e var).
+End language.
