src/Reflection/MapCastInterp.v
@@ -1,0 +1,188 @@
+Require Import Crypto.Reflection.Syntax.
+Require Import Crypto.Reflection.Wf.
+Require Import Crypto.Reflection.SmartMap.
+Require Import Crypto.Reflection.ExprInversion.
+Require Import Crypto.Reflection.MapCast.
+Require Import Crypto.Reflection.Relations.
+Require Import Crypto.Reflection.WfProofs.
+Require Import Crypto.Reflection.WfInversion.
+Require Import Crypto.Util.Sigma.
+Require Import Crypto.Util.Prod.
+Require Import Crypto.Util.Option.
+Require Import Crypto.Util.Tactics.BreakMatch.
+Require Import Crypto.Util.Tactics.SpecializeBy.
+Require Import Crypto.Util.Tactics.DestructHead.
+
+Local Open Scope ctype_scope.
+Local Open Scope expr_scope.
+Section language.
+  Context {base_type_code : Type}
+          {interp_base_type1 : base_type_code -> Type}
+          {interp_base_type2 : base_type_code -> Type}
+          {op : flat_type base_type_code -> flat_type base_type_code -> Type}
+          (interp_op1 : forall src dst, op src dst -> interp_flat_type interp_base_type1 src -> interp_flat_type interp_base_type1 dst)
+          (interp_op2 : forall src dst, op src dst -> interp_flat_type interp_base_type2 src -> interp_flat_type interp_base_type2 dst)
+          (failv : forall {var t}, @exprf base_type_code op var (Tbase t)).
+  Context (transfer_op : forall ovar src1 dst1 src2 dst2
+                                (opc1 : op src1 dst1)
+                                (opc2 : op src2 dst2)
+                                (args1' : @exprf base_type_code op ovar src1)
+                                (args2 : interp_flat_type interp_base_type2 src2),
+              @exprf base_type_code op ovar dst1).
+
+  Context (bound_is_good : forall t, interp_base_type2 t -> Prop).
+  Local Notation bounds_are_good
+    := (@interp_flat_type_rel_pointwise0 _ _ bound_is_good).
+
+  Fixpoint bounds_are_recursively_good {t} (e : exprf base_type_code op t) : Prop
+    := match e with
+       | LetIn tx ex tC eC
+         => @bounds_are_recursively_good tx ex
+            /\ @bounds_are_recursively_good tC (eC (interpf interp_op2 ex))
+       | Op t1 tR opc args as e'
+         => @bounds_are_recursively_good _ args
+            /\ bounds_are_good (interpf interp_op2 e')
+       | TT => True
+       | Var t v => bound_is_good _ v
+       | Pair tx ex ty ey
+         => @bounds_are_recursively_good _ ex
+            /\ @bounds_are_recursively_good _ ey
+       end.
+  Lemma bounds_are_good_when_recursively_good {t} e
+    : @bounds_are_recursively_good t e -> bounds_are_good (interpf interp_op2 e).
+  Proof.
+    induction e; simpl; unfold LetIn.Let_In; intuition auto.
+  Qed.
+  Local Hint Resolve bounds_are_good_when_recursively_good.
+
+  Context (interpf_transfer_op
+           : forall G t tR opc ein eout ebounds,
+              wff G ein ebounds
+              -> interpf interp_op1 ein = interpf interp_op1 eout
+              -> bounds_are_recursively_good ebounds
+              -> bounds_are_good (interp_op2 t tR opc (interpf interp_op2 ebounds))
+              -> interpf interp_op1 (transfer_op interp_base_type1 t tR t tR opc opc eout (interpf interp_op2 ebounds))
+                 = interpf interp_op1 (Op opc ein)).
+
+  Local Notation mapf_interp_cast
+    := (@mapf_interp_cast
+          base_type_code base_type_code interp_base_type2
+          op op interp_op2 failv
+          transfer_op).
+  Local Notation map_interp_cast
+    := (@map_interp_cast
+          base_type_code base_type_code interp_base_type2
+          op op interp_op2 failv
+          transfer_op).
+  Local Notation MapInterpCast
+      := (@MapInterpCast
+            base_type_code interp_base_type2
+            op interp_op2 failv
+            transfer_op).
+
+  (* Local *) Hint Resolve <- List.in_app_iff.
+
+  Local Ltac break_t
+    := first [ progress subst
+             | progress inversion_wf
+             | progress invert_expr_subst
+             | progress inversion_sigma
+             | progress inversion_prod
+             | progress destruct_head sig
+             | progress destruct_head sigT
+             | progress destruct_head ex
+             | progress destruct_head and
+             | progress destruct_head prod
+             | progress break_match_hyps ].
+
+  Local Ltac fin_False :=
+    lazymatch goal with
+    | [ H : False |- _ ] => exfalso; assumption
+    end.
+
+  Local Ltac fin_t0 :=
+    solve [ constructor; eauto
+          | eauto
+          | auto
+          | hnf; auto ].
+
+  Local Ltac handle_list_t :=
+    match goal with
+    | _ => progress cbv [LetIn.Let_In duplicate_types] in *
+    | [ H : List.In _ (_ ++ _) |- _ ] => apply List.in_app_or in H
+    | [ H : List.In _ (List.map _ _) |- _ ]
+      => rewrite List.in_map_iff in H
+    | _ => rewrite <- flatten_binding_list_flatten_binding_list2
+    | [ H : appcontext[flatten_binding_list2] |- _ ]
+      => rewrite <- flatten_binding_list_flatten_binding_list2 in H
+    | [ H : context[flatten_binding_list (SmartVarfMap _ _) (SmartVarfMap _ _)] |- _ ]
+      => rewrite flatten_binding_list_SmartVarfMap in H
+    | [ H : context[flatten_binding_list2 (SmartVarfMap _ _) (SmartVarfMap _ _)] |- _ ]
+      => rewrite flatten_binding_list2_SmartVarfMap in H
+    | [ H : context[flatten_binding_list2 (SmartVarfMap _ _) _] |- _ ]
+      => rewrite flatten_binding_list2_SmartVarfMap1 in H
+    | [ H : context[flatten_binding_list2 _ (SmartVarfMap _ _)] |- _ ]
+      => rewrite flatten_binding_list2_SmartVarfMap2 in H
+    | _ => rewrite <- flatten_binding_list_flatten_binding_list2
+    | _ => rewrite List.in_map_iff
+    end.
+
+  Local Ltac wff_t :=
+    match goal with
+    | [ |- wff _ _ _ ] => constructor
+    | [ H : _ |- wff _ (mapf_interp_cast _ _ _) (mapf_interp_cast _ _ _) ]
+      => eapply H; eauto; []; clear H
+    | _ => solve [ eauto using wff_in_impl_Proper ]
+    end.
+
+  Local Ltac misc_t :=
+    match goal with
+    | _ => progress specialize_by eauto
+    | [ |- exists _, _ ]
+      => eexists (existT _ _ _)
+    | [ |- _ /\ _ ] => split
+    | [ H : _ = _ |- _ ] => rewrite H
+    end.
+
+  Local Ltac t_step :=
+    first [ intro
+          | fin_False
+          | progress break_t
+          | fin_t0
+          | progress simpl in *
+          | wff_t
+          | handle_list_t
+          | progress destruct_head' or
+          | misc_t ].
+
+  Lemma interpf_mapf_interp_cast
+        G
+        {t1} e1 ebounds
+        (Hgood : bounds_are_recursively_good ebounds)
+        (Hwf : wff G e1 ebounds)
+    : interpf interp_op1 (@mapf_interp_cast interp_base_type1 t1 e1 t1 ebounds)
+      = interpf interp_op1 e1.
+  Proof. induction Hwf; repeat t_step. Qed.
+
+  Local Hint Resolve interpf_mapf_interp_cast.
+
+  Lemma interp_map_interp_cast
+        {t1} e1 ebounds
+        args2
+        (Hgood : bounds_are_recursively_good (invert_Abs ebounds args2))
+        (Hwf : wf e1 ebounds)
+    : forall x,
+      interp interp_op1 (@map_interp_cast interp_base_type1 t1 e1 t1 ebounds args2) x
+      = interp interp_op1 e1 x.
+  Proof. destruct Hwf; intro; eapply interpf_mapf_interp_cast; eauto. Qed.
+
+  Lemma InterpMapInterpCast
+        {t} e
+        args
+        (Hwf : Wf e)
+        (Hgood : bounds_are_recursively_good (invert_Abs (e interp_base_type2) args))
+    : forall x,
+      Interp interp_op1 (@MapInterpCast t e args) x
+      = Interp interp_op1 e x.
+  Proof. apply interp_map_interp_cast; auto. Qed.
+End language.
