src/Reflection/MapCastWithCastOpWf.v
@@ -1,0 +1,348 @@
+Require Import Crypto.Reflection.Syntax.
+Require Import Crypto.Reflection.Wf.
+Require Import Crypto.Reflection.SmartMap.
+Require Import Crypto.Reflection.ExprInversion.
+Require Import Crypto.Reflection.MapCastWithCastOp.
+Require Import Crypto.Reflection.MapCastWf.
+Require Import Crypto.Reflection.WfProofs.
+Require Import Crypto.Reflection.WfInversion.
+Require Import Crypto.Util.Sigma.
+Require Import Crypto.Util.Prod.
+Require Import Crypto.Util.Option.
+Require Import Crypto.Util.Equality.
+Require Import Crypto.Util.Tactics.BreakMatch.
+Require Import Crypto.Util.Tactics.DestructHead.
+Require Import Crypto.Util.Tactics.SpecializeBy.
+
+Local Open Scope ctype_scope.
+Local Open Scope expr_scope.
+Section language.
+  Context {base_type_code : Type}
+          {interp_base_type : base_type_code -> Type}
+          {op : flat_type base_type_code -> flat_type base_type_code -> Type}
+          (interp_op2 : forall src dst, op src dst -> interp_flat_type interp_base_type src -> interp_flat_type interp_base_type dst)
+          (base_type_code_beq : base_type_code -> base_type_code -> bool)
+          (base_type_code_bl : forall x y, base_type_code_beq x y = true -> x = y)
+          (base_type_code_lb : forall x y, x = y -> base_type_code_beq x y = true)
+          (failv : forall {var t}, @exprf base_type_code op var (Tbase t))
+          (new_base_type : forall t, interp_base_type t -> base_type_code)
+          (Cast : forall var t1 t2, @exprf base_type_code op var (Tbase t1)
+                                    -> @exprf base_type_code op var (Tbase t2))
+          (is_cast : forall t1 t2, op t1 t2 -> bool).
+  Local Notation new_flat_type (*: forall t, interp_flat_type interp_base_type2 t -> flat_type base_type_code1*)
+    := (@SmartFlatTypeMap2 _ _ interp_base_type (fun t v => Tbase (new_base_type t v))).
+  Context (new_op : forall ovar src1 dst1 src2 dst2 (opc1 : op src1 dst1) (opc2 : op src2 dst2)
+                           args2,
+              option { new_src : _ & (@exprf base_type_code op ovar new_src
+                                      -> @exprf base_type_code op ovar (new_flat_type (interpf interp_op2 (Op opc2 args2))))%type }).
+  Local Notation SmartFail
+    := (SmartValf _ (@failv _)).
+  Local Notation failf t (* {t} : @exprf base_type_code1 op1 ovar t*)
+    := (SmartPairf (SmartFail t)).
+  Local Notation mapf_interp_cast_with_cast_op
+    := (@mapf_interp_cast_with_cast_op
+          base_type_code base_type_code interp_base_type
+          op op interp_op2
+          base_type_code_beq base_type_code_bl
+          failv new_base_type Cast is_cast new_op).
+  Local Notation map_interp_cast_with_cast_op
+    := (@map_interp_cast_with_cast_op
+          base_type_code base_type_code interp_base_type
+          op op interp_op2
+          base_type_code_beq base_type_code_bl
+          failv new_base_type Cast is_cast new_op).
+  Local Notation bound_op
+    := (@bound_op
+          base_type_code base_type_code interp_base_type
+          op op interp_op2
+          base_type_code_beq base_type_code_bl
+          failv new_base_type Cast is_cast new_op).
+  Local Notation bound_var
+    := (@bound_var
+          base_type_code
+          op
+          base_type_code_beq base_type_code_bl
+          failv Cast is_cast).
+  Local Notation bound_var1
+    := (@bound_var1
+          base_type_code base_type_code interp_base_type
+          op
+          base_type_code_beq base_type_code_bl
+          failv new_base_type Cast is_cast).
+  Local Notation bound_var2
+    := (@bound_var2
+          base_type_code base_type_code interp_base_type
+          op op interp_op2
+          base_type_code_beq base_type_code_bl
+          failv new_base_type Cast is_cast).
+
+  Local Notation interp_flat_type_ivarf_wff G a b
+    := (forall t x y,
+           List.In (existT _ t (x, y)%core) (flatten_binding_list a b)
+           -> wff G x y)
+         (only parsing).
+
+  Section with_var.
+    Context {ovar1 ovar2 : base_type_code -> Type}.
+    Local Notation ivar1 t := (@exprf base_type_code op ovar1 (Tbase t)) (only parsing).
+    Local Notation ivar2 t := (@exprf base_type_code op ovar2 (Tbase t)) (only parsing).
+    Local Notation ivarf1 := (fun t => ivar1 t).
+    Local Notation ivarf2 := (fun t => ivar2 t).
+
+    Local Notation G1eTf
+      := (fun t : base_type_code => interp_flat_type ivarf1 (Tbase t) * interp_flat_type ivarf2 (Tbase t))%type.
+    Local Notation G2eTf
+      := (fun t : base_type_code => ovar1 t * ovar2 t)%type.
+    Local Notation GbeTf
+      := (fun t : base_type_code => interp_flat_type ivarf1 (Tbase t) * interp_base_type t)%type.
+
+    Local Hint Constructors Wf.wff.
+
+    Lemma wff_failf G t
+          (wff_failv : forall T, wff G (failv ovar1 T) (failv ovar2 T))
+      : wff (t:=t) (var1:=ovar1) (var2:=ovar2) G (failf t) (failf t).
+    Proof.
+      clear -wff_failv.
+      induction t; simpl; rewrite ?SmartPairf_Pair; eauto; constructor.
+    Qed.
+
+    Local Hint Resolve wff_failf.
+
+    Local Ltac t_step :=
+      match goal with
+      | _ => progress simpl
+      | _ => progress break_innermost_match
+      | _ => solve [ constructor | eauto ]
+      | [ |- ?f _ match ?H with eq_refl => ?v1 end match ?H with eq_refl => ?v2 end ]
+        => rewrite (@commute_eq_match2 _ _ _ _ f _ _ H v1 v2)
+      | _ => rewrite eq_match_const
+      | [ wff_Cast : forall t1 t2 a b, wff _ _ _ -> wff _ (Cast _ _ _ _) (Cast _ _ _ _)
+                                       |- wff _ (Cast _ _ _ _) (Cast _ _ _ _) ]
+        => apply wff_Cast
+      | _ => rewrite SmartPairf_Pair
+      | _ => progress specialize_by auto
+      | [ Hxy : forall k, List.In k _ -> List.In k ?G |- List.In _ ?G ]
+        => apply Hxy
+      | [ |- context[List.In _ (_ ++ _)] ] => rewrite List.in_app_iff
+      | [ |- wff _ _ _ ] => constructor
+      | [ |- wff _ _ _ ] => eapply wff_in_impl_Proper; [ solve [ eauto with nocore ] | ]
+      | _ => intro
+      end.
+
+    Lemma wff_VarBound G a b x y
+          (wff_failv : forall T, wff G (failv ovar1 T) (failv ovar2 T))
+          (wff_Cast : forall t1 t2 a b, wff G a b -> wff G (Cast ovar1 t1 t2 a)
+                                                         (Cast ovar2 t1 t2 b))
+          (Hxy : forall k, List.In k (flatten_binding_list x y) -> List.In k G)
+      : wff G
+            (VarBound failv Cast (var:=ovar1) a b x)
+            (VarBound failv Cast (var:=ovar2) a b y).
+    Proof.
+      clear -wff_failv wff_Cast Hxy.
+      revert dependent b; induction a;
+        repeat match goal with
+               | _ => progress t_step
+               | [ H : _ |- _ ] => apply H
+               end.
+    Qed.
+
+    Lemma wff_SmartBound G t1 t2 e1 e2
+          (wff_failv : forall T, wff G (failv ovar1 T) (failv ovar2 T))
+          (wff_Cast : forall G t1 t2 a b, wff G a b -> wff G (Cast ovar1 t1 t2 a)
+                                                         (Cast ovar2 t1 t2 b))
+          (Hwf : wff (t:=t1) G e1 e2)
+      : wff (t:=t2) G
+            (SmartBound (var:=ovar1) base_type_code_beq base_type_code_bl failv Cast is_cast e1)
+            (SmartBound (var:=ovar2) base_type_code_beq base_type_code_bl failv Cast is_cast e2).
+    Proof.
+      clear -wff_failv wff_Cast Hwf.
+      revert dependent t2; induction Hwf; intros; specialize_by auto;
+        induction t2;
+        repeat match goal with
+               | [ |- wff _ (VarBound _ _ _ _ _) (VarBound _ _ _ _ _) ]
+                 => apply wff_VarBound
+               | _ => progress t_step
+               end.
+    Qed.
+
+    Section with_assumptions.
+      Context (wff_failv : forall G T, wff G (failv ovar1 T) (failv ovar2 T))
+              (wff_Cast : forall G t1 t2 a b,
+                  wff G a b -> wff G (Cast ovar1 t1 t2 a) (Cast ovar2 t1 t2 b))
+              (wff_new_op
+               : forall G src1 dst1 src2 dst2 opc1 opc2 args0
+                        (v1 : forall t, exprf _ _ t)
+                        (v2 : forall t, exprf _ _ t),
+                  (forall t, wff G (v1 t) (v2 t))
+                  -> match new_op ovar1 src1 dst1 src2 dst2 opc1 opc2 args0, new_op ovar2 src1 dst1 src2 dst2 opc1 opc2 args0 with
+                     | Some f, Some g => wff G (projT2 f (v1 (projT1 f))) (projT2 g (v2 (projT1 g)))
+                     | None, None => True
+                     | Some _, None | None, Some _ => False
+                     end).
+
+      Lemma wff_bound_op
+            G src1 dst1 src2 dst2 opc1 opc2 args2 e1 e2
+            (Hwf : wff G (var1:=ovar1) (var2:=ovar2) e1 e2)
+        : wff G
+              (@bound_op ovar1 src1 dst1 src2 dst2 opc1 opc2 args2 e1)
+              (@bound_op ovar2 src1 dst1 src2 dst2 opc1 opc2 args2 e2).
+      Proof.
+        specialize (wff_new_op G src1 dst1 src2 dst2 opc1 opc2 args2).
+        unfold MapCastWithCastOp.bound_op.
+        repeat match goal with
+               | _ => solve [ eauto using wff_SmartBound | exfalso; assumption ]
+               | _ => progress specialize_by eauto
+               | [ |- wff ?G (projT2 ?f ?a) (projT2 ?g ?b) ]
+                 => let a := match (eval pattern (projT1 f) in a) with ?a _ => a end in
+                    let b := match (eval pattern (projT1 g) in b) with ?b _ => b end in
+                    specialize (wff_new_op a b)
+               | _ => progress break_match_step ltac:(fun _ => idtac)
+                   | [ |- wff ?G _ _ ] => specialize (wff_new_op (fun t => failf t) (fun t => failf t))
+               end.
+      Qed.
+
+      Local Hint Resolve wff_bound_op.
+
+      Lemma wff_bound_var
+            G tx1 tx2 tC1 f1 f2 e1 e2
+            (Hwfe : interp_flat_type_ivarf_wff G e1 e2)
+            (Hwff : forall x y, interp_flat_type_ivarf_wff G x y -> wff G (f1 x) (f2 y))
+        : wff G
+              (@bound_var ovar1 tx1 tx2 tC1 f1 e1)
+              (@bound_var ovar2 tx1 tx2 tC1 f2 e2).
+      Proof.
+        revert dependent tx1.
+        induction tx2;
+          repeat match goal with
+                 | _ => progress subst
+                 | _ => progress inversion_sigma
+                 | _ => progress inversion_prod
+                 | _ => progress destruct_head' ex
+                 | _ => progress destruct_head' and
+                 | _ => progress break_match_step ltac:(fun _ => idtac)
+                 | [ H : False |- _ ] => exfalso; assumption
+                 | [ H : context[List.In _ (_ ++ _)] |- _ ]
+                   => rewrite List.in_app_iff in H
+                 | [ H : context[List.In _ (_ ++ _)] |- _ ]
+                   => setoid_rewrite List.in_app_iff in H
+                 | [ H : forall x y, _ -> wff ?G (?f1 _) (?f2 _) |- wff ?G (?f1 _) (?f2 _) ]
+                   => apply H; clear H
+                 | [ |- wff _ (SmartBound _ _ _ _ _ _) (SmartBound _ _ _ _ _ _) ]
+                   => apply wff_SmartBound
+                 | _ => intro
+                 | _ => solve [ eauto ]
+                 | _ => progress simpl in *
+                 | _ => progress destruct_head' or
+                 | [ H : context[flatten_binding_list (SmartValf _ _ _) (SmartValf _ _ _)] |- _ ]
+                   => rewrite flatten_binding_list_SmartValf in H
+                 | [ H : List.In _ (List.map _ _) |- _ ]
+                   => rewrite List.in_map_iff in H
+                 | [ H : _ |- wff _ (bound_var _ _ _ _ _) (bound_var _ _ _ _ _) ]
+                   => apply H; clear H
+                 end.
+      Qed.
+
+      Local Hint Resolve wff_bound_var.
+
+      Lemma wff_bound_var1
+            G t x1 x2 v
+            (Hwf : wff G x1 x2)
+        : wff G
+              (@bound_var1 ovar1 t t x1 v)
+              (@bound_var1 ovar2 t t x2 v).
+      Proof.
+        apply wff_bound_var;
+          repeat match goal with
+                 | _ => intro
+                 | _ => assumption
+                 | [ H : False |- _ ] => exfalso; assumption
+                 | _ => progress subst
+                 | _ => progress inversion_sigma
+                 | _ => progress inversion_prod
+                 | _ => progress simpl in *
+                 | _ => progress destruct_head' or
+                 | _ => solve [ eauto ]
+                 end.
+      Qed.
+
+      Local Hint Resolve wff_bound_var1.
+
+      Lemma wff_bound_var2
+            G tx tC ex' eC' f g v1 v2
+            (Hwfg : forall a b,
+                interp_flat_type_ivarf_wff G a b
+                -> wff G (f a) (g b))
+            (Hwfv : wff (op:=op) G (SmartVarf v1) (SmartVarf v2))
+        : wff G
+              (@bound_var2 ovar1 tx tx tC ex' eC' f v1)
+              (@bound_var2 ovar2 tx tx tC ex' eC' g v2).
+      Proof.
+        apply wff_bound_var;
+          repeat match goal with
+                 | _ => intro
+                 | _ => assumption
+                 | [ H : False |- _ ] => exfalso; assumption
+                 | _ => progress subst
+                 | _ => progress inversion_sigma
+                 | _ => progress inversion_prod
+                 | _ => progress destruct_head' ex
+                 | _ => progress destruct_head' and
+                 | _ => progress destruct_head' sigT
+                 | _ => progress destruct_head' prod
+                 | _ => progress simpl in *
+                 | _ => progress destruct_head' or
+                 | _ => solve [ eauto using In_G_wff_SmartVarf, wff_in_impl_Proper ]
+                 | [ H : context[flatten_binding_list (SmartVarfMap _ _) (SmartVarfMap _ _)] |- _ ]
+                   => rewrite flatten_binding_list_SmartVarfMap in H
+                 | [ H : List.In _ (List.map _ _) |- _ ]
+                   => rewrite List.in_map_iff in H
+                 end.
+      Qed.
+
+      Local Hint Resolve wff_bound_var2.
+
+      Lemma wf_map_interp_cast_with_cast_op
+            {t1} e1 e2 ebounds args
+            (Hwf_bounds : wf e1 ebounds)
+            (Hwf : wf e1 e2)
+        : wf (@map_interp_cast_with_cast_op ovar1 t1 e1 t1 ebounds args)
+             (@map_interp_cast_with_cast_op ovar2 t1 e2 t1 ebounds args).
+      Proof.
+        eapply wf_map_interp_cast; eauto.
+      Qed.
+    End with_assumptions.
+  End with_var.
+
+  Section gen.
+    Context (wff_failv : forall ovar1 ovar2 G T, wff G (failv ovar1 T) (failv ovar2 T))
+            (wff_Cast : forall ovar1 ovar2 G t1 t2 a b,
+                wff G a b -> wff G (Cast ovar1 t1 t2 a) (Cast ovar2 t1 t2 b))
+            (wff_new_op
+             : forall ovar1 ovar2 G src1 dst1 src2 dst2 opc1 opc2 args0
+                      (v1 : forall t, exprf _ _ t)
+                      (v2 : forall t, exprf _ _ t),
+                (forall t, wff G (v1 t) (v2 t))
+                -> match new_op ovar1 src1 dst1 src2 dst2 opc1 opc2 args0, new_op ovar2 src1 dst1 src2 dst2 opc1 opc2 args0 with
+                   | Some f, Some g => wff G (projT2 f (v1 (projT1 f))) (projT2 g (v2 (projT1 g)))
+                   | None, None => True
+                   | Some _, None | None, Some _ => False
+                   end).
+
+    Local Notation MapInterpCastWithCastOp
+      := (@MapInterpCastWithCastOp
+            base_type_code interp_base_type
+            op interp_op2
+            base_type_code_beq base_type_code_bl
+            failv new_base_type Cast is_cast new_op).
+
+    Lemma WfMapInterpCastWithCastOp
+          {t} e
+          args
+          (Hwf : Wf e)
+      : Wf (@MapInterpCastWithCastOp t e args).
+    Proof.
+      intros ??; apply wf_map_interp_cast_with_cast_op; eauto;
+        apply wff_new_op.
+    Qed.
+  End gen.
+End language.
