src/Specific/GF25519Reflective/Reified/AddCoordinates.v
@@ -7,7 +7,6 @@ Require Import Crypto.Reflection.Syntax.
 Require Import Crypto.Reflection.SmartMap.
 Require Import Crypto.Reflection.ExprInversion.
 Require Import Crypto.Reflection.Relations.
-Require Import Crypto.Reflection.Application.
 Require Import Crypto.Reflection.Linearize.
 Require Import Crypto.Reflection.Z.Interpretations64.
 Require Crypto.Reflection.Z.Interpretations64.Relations.
